pass w/ new definitions

src/Iris/Algebra/Heap.lean
@@ -23,217 +23,176 @@ Note: There are three definitions of equivalence in this file
 -/
 
 
+-- TODO: Reuse set theory as defined in ghost maps PR, and delete this
+def set_disjoint {X : Type _} (S1 S2 : X → Prop) : Prop := ∀ x : X, ¬(S1 x ∧ S2 x)
+def set_union {X : Type _} (S1 S2 : X → Prop) : X → Prop := fun x => S1 x ∨ S2 x
+def set_included {X : Type _} (S1 S2 : X → Prop) : Prop := ∀ x, S1 x → S2 x
 
-/- # Datatype and CMRA for a generic heap-like structure. -/
+/-! # StoreLike -/
 
 /-- The type `T` can store and retrieve keys of type `K` and obtain values of type `V`. -/
-class StoreLike (T : Type _) (K V : outParam (Type _)) where
+class Store (T : Type _) (K V : outParam (Type _)) where
   get : T → K → V
   set : T → K → V → T
-  ofFun : (K → V) → T
-export StoreLike (get set)
-
-/-- `T`'s store and retrieve operations behave like a classical store. -/
-class Store (T : Type _) (K V : outParam (Type _)) extends StoreLike T K V where
+  merge (op : V → V → V) : T → T → T
   get_set_eq {t k k' v} : k = k' → get (set t k v) k' = v
   get_set_ne {t k k' v} : k ≠ k' → get (set t k v) k' = get t k'
-  /-- One-sided inverse between get and ofFun. The other direction does not need to hold. -/
-  ofFun_get {f} : get (ofFun f) = f
-
-/-- Two stores are (pointwise) equivalent -/
-def Store.Equiv [StoreLike T K V] (t1 t2 : T) : Prop := get t1 = get t2
-
-/-- Each value of `T` uniquely represents a function `K → V`. -/
-class IsStoreIso (T : Type _) (K V : outParam (Type _)) [I : Store T K V] where
-  get_ofFun t : I.toStoreLike.ofFun (get t) = t
-
-def StoreLike.map [StoreLike T1 K V1] [StoreLike T2 K V2] (t : T1) (f : V1 → V2) : T2 :=
-  StoreLike.ofFun (fun i => f <| StoreLike.get t i)
-
-def StoreLike.merge [StoreLike T K V] (op : V → V → V) (t1 t2 : T) : T :=
-  StoreLike.ofFun <| (fun k => op (StoreLike.get t1 k) (StoreLike.get t2 k))
+  get_merge {t1 t2 k v1 v2} : get t1 k = v1 → get t2 k = v2 → get (merge op t1 t2) k = op v1 v2
+export Store (get set merge get_set_eq get_set_ne get_merge)
 
 /-- An (index-dependent) predicate holds at every member of the store. -/
-def StoreLike.all [StoreLike T K V] (P : K → V → Prop) : T → Prop :=
-  fun t => ∀ k, P k (StoreLike.get t k)
+def Store.all [Store T K V] (P : K → V → Prop) : T → Prop :=
+  fun t => ∀ k, P k (get t k)
+
+/-- Two Stores are pointwise equivalent. -/
+def Store.Equiv [Store T K V] (t1 t2 : T) : Prop := get t1 = get t2
+
+instance Equiv_trans [Store T K V] : Trans (Store.Equiv : T → T → Prop) (Store.Equiv : T → T → Prop) (Store.Equiv : T → T → Prop) where
+  trans := by simp_all [Store.Equiv]
+
+/-- RepFunStore: The type T can represent all functions that satisfy Rep  -/
+class RepFunStore (T : Type _) (K V : outParam (Type _)) [Store T K V] where
+  rep : (K → V) → Prop
+  rep_get (t : T) : rep (get t)
+  ofFun : { f : K → V // rep f } → T
+  get_ofFun: get (ofFun f) = f
+export RepFunStore (rep rep_get ofFun get_ofFun)
+
+/-- IsoFunStore: The type T is isomorphic the type of functions {f : Rep f}. -/
+class IsoFunStore (T : Type _) (K V : outParam (Type _)) [Store T K V] extends RepFunStore T K V where
+  ofFun_get {t : T} : ofFun ⟨get t, rep_get t⟩ = t
+export IsoFunStore (ofFun_get)
+
+theorem IsStoreIso.ext [Store T K V] [IsoFunStore T K V] {t1 t2 : T}
+    (H : ∀ k, get t1 k = get t2 k) : t1 = t2 := by
+  rw [← ofFun_get (t := t1), ← ofFun_get (t := t2)]
+  congr 2
+  exact funext H
+
+/-- When the type is a StoreIso, equality coincides with pointwise equality ([2] -> [3]). -/
+theorem IsStoreIso.store_eq_of_Equiv [Store T K V] [IsoFunStore T K V] {t1 t2 : T} :
+    Store.Equiv t1 t2 → t1 = t2 := (IsStoreIso.ext <| fun k => congrFun · k)
+
+class HasStoreMap (T1 T2 : Type _) (K V1 V2 : outParam (Type _)) [Store T1 K V1] [Store T2 K V2] where
+  /-- Map a function that depends on the elemet across the entire structure  -/
+  dmap (f : K → V1 → V2) : T1 → T2
+  get_dmap : Store.get (dmap f t) k = f k (Store.get t k)
+export HasStoreMap (dmap get_dmap)
+
+abbrev HasStoreMap.map (f : V1 → V2) [Store T1 K V1] [Store T2 K V2] [HasStoreMap T1 T2 K V1 V2] : T1 → T2 :=
+  HasStoreMap.dmap (fun (_ : K) => f)
+
+/-- HeapLike: The type T behaves like a partial store with keys K and values V for all value types V. -/
+class Heap (T : Type _ → Type _) (K : outParam (Type _)) where
+  [isStore : ∀ {V : Type _}, Store (T V) K (Option V)]
+  [hasStoreMap : ∀ {V1 V2 : Type _}, HasStoreMap (T V1) (T V2) K (Option V1) (Option V2)]
+  empty (V : Type _) : T V
+  get_empty : get (empty V : T V) k = none
+export Heap (empty isStore hasStoreMap get_empty)
+
+attribute [instance] Heap.isStore
+attribute [instance] Heap.hasStoreMap
 
 /-- Lift a predicate on store values to a predicate on heap values, which is true for undefined entries. -/
-abbrev liftHeapPred (P : K → V → Prop) (k : K) : Option V → Prop
-  | .some v => P k v
-  | .none => True
+def toHeapPred (P : K → V → Prop) (k : K) : Option V → Prop
+| .some v => P k v
+| .none => True
 
-class WithPoints (T : Type _) (K V : outParam (Type _)) where
-  point : K → V → T
-
-class HeapLike (T : Type _) (K V : outParam (Type _)) extends StoreLike T K (Option V)
-
-/-- A Heap with a partial `fresh` function -/
-class Alloc (T : Type _) (K V : outParam (Type _)) extends HeapLike T K V where
-  hasRoom : T → Prop
-  fresh : {t : T} → hasRoom t → K
-  fresh_get {H : hasRoom t} : get t (fresh H) = none
-
-/-- A type is HeapLike when it behaves like store for Optional values -/
-class Heap (T : Type _) (K V : outParam (Type _))
-    extends HeapLike T K V, Store T K (Option V), WithPoints T K (Option V) where
-  point_get_eq {k k' v} : k = k' → get (point k v) k' = v
-  point_get_ne {k k' v} : k ≠ k' → get (point k v) k' = none
-
-/-- A Heap whose `fresh` function is total -/
-class AllocHeap (T : Type _) (K V : outParam (Type _)) extends Heap T K V, Alloc T K V where
-  hasRoom_set_fresh {H : hasRoom t} {v} : hasRoom (set t (fresh H) v)
+/-- The heap of a single point -/
+def Heap.point [Heap T K] (k : K) (v : Option V) : T V := Store.set (empty V) k v
 
 /-- Delete an element from a heap by setting its value to .none -/
-abbrev HeapLike.delete [HeapLike T K V] (t : T) (k : K) : T := StoreLike.set t k .none
-
-/-- A heap is empty when its get function is .none. -/
-abbrev HeapLike.empty [HeapLike T K V] : T := StoreLike.ofFun (fun _ => .none)
+def Heap.delete [Heap T K] (t : T V) (k : K) : T V := Store.set t k none
 
 /-- The domain of a heap is the set of keys that map to .some values. -/
-abbrev HeapLike.dom [HeapLike T K V] : T → K → Prop := fun t k => (StoreLike.get t k).isSome
+def Heap.dom [Heap T K] (t : T V) : K → Prop := fun k => (Store.get t k).isSome
 
-/-- Value-generic heap, ie. a higher-order type that is heap-like at every type.
-For heaps whose representation internalizes the type which it contains, (for example, lists,
-trees, functions) this is probably the class you want. -/
-abbrev HeapF (H : Type _ → Type _) (K : outParam (Type _)) :=
-  ∀ T : Type _, HeapLike (H T) K T
+@[simp] def Heap.union [Heap T K] (t1 t2 : T V) : T V :=
+  let F : Option V → Option V → Option V
+  | .some v1 => fun _ => v1
+  | .none => id
+  Store.merge F t1 t2
 
-theorem Store.get_merge [Store T K V] {op : V → V → V} (t1 t2 : T) (k : K) :
-    StoreLike.get (StoreLike.merge op t1 t2) k = op (StoreLike.get t1 k) (StoreLike.get t2 k) := by
-  unfold StoreLike.merge; rw [Store.ofFun_get]
+theorem Heap.point_get_eq [Heap T K] : k = k' → Store.get (Heap.point k v : T V) k' = v := by
+  intro H; unfold point; rw [@get_set_eq]; exact H
 
-theorem Store.get_map [StoreLike T1 K V1] [Store T2 K V2] {t : T1} {f : V1 → V2} {k : K} :
-    StoreLike.get (StoreLike.map t f : T2) k = f (StoreLike.get t k) := by
-  unfold StoreLike.map; rw [Store.ofFun_get]
+theorem Heap.point_get_ne [Heap T K] : k ≠ k' → Store.get (Heap.point k v : T V) k' = none := by
+  intro H; unfold point; rw [@get_set_ne, get_empty]; exact H
 
-theorem IsStoreIso.ext [Store T K V] [IsStoreIso T K V] {t1 t2 : T} (H : ∀ k, get t1 k = get t2 k) : t1 = t2 := by
-  rw [← IsStoreIso.get_ofFun t1, ← IsStoreIso.get_ofFun t2]; refine congrArg ?_ (funext H)
+/-- An AllocHeap is a heap which can allocate elements under some condition. -/
+class AllocHeap (T : Type _ → Type _) (K : outParam (Type _)) extends Heap T K where
+  notFull : T V → Prop
+  fresh {t : T V} : notFull t → K
+  get_fresh  {H : notFull t} : Store.get t (fresh H) = none
+export AllocHeap (notFull fresh get_fresh)
 
-theorem IsStoreIso.store_eq_of_Equiv [Store T K V] [IsStoreIso T K V] {t1 t2 : T} :
-    Store.Equiv t1 t2 → t1 = t2 :=
-  (IsStoreIso.ext <| fun k => congrFun · k)
-
-/-- Wrapper type for functions with the Store OFE -/
-@[ext] structure StoreO (T : Type _) where car : T
+/-- An UnboundeHeap is a heap which can allocate an unbounded number of elements starting at empty. -/
+class UnboundedHeap (T : Type _ → Type _) (K : outParam (Type _)) extends AllocHeap T K where
+  notFull_empty : notFull (empty V : T V)
+  notFull_set_fresh {H : notFull t} : notFull (Store.set t (fresh H) v)
+export UnboundedHeap (notFull_empty notFull_set_fresh)
 
 section ofe
 
-open OFE 
+open OFE
 
 /-- The OFE on StoreO is the discrete function OFE on its .get function. -/
-instance StoreO_OFE [StoreLike T K V] [OFE V] : OFE (StoreO T) where
-  Equiv s0 s1  := StoreLike.get s0.1 ≡ StoreLike.get s1.1
-  Dist n s0 s1 := StoreLike.get s0.1 ≡{n}≡ StoreLike.get s1.1
+instance Store_OFE [Store T K V] [OFE V] : OFE T where
+  Equiv s0 s1  := Store.get s0 ≡ Store.get s1
+  Dist n s0 s1 := Store.get s0 ≡{n}≡ Store.get s1
   dist_eqv     := ⟨fun _ => .of_eq rfl, (·.symm), (·.trans ·)⟩
   equiv_dist   := equiv_dist
   dist_lt      := dist_lt
 
-@[simp] def StoreO.toMap [StoreLike T K V] [OFE V] : (StoreO T) -n> (K → V) where
-  f x := StoreLike.get <| StoreO.car x
+@[simp] def Store.toMap [Store T K V] [OFE V] : T -n> (K → V) where
+  f x := Store.get x
   ne.1 {_ _ _} H k := H k
 
-@[simp] def StoreO.ofMap [Store T K V] [OFE V] : (K → V) -n> (StoreO T) where
-  f x := StoreO.mk <| StoreLike.ofFun x
-  ne.1 {_ _ _} H k := by rw [Store.ofFun_get, Store.ofFun_get]; exact H k
+@[simp] def Store.ofMap [Store T K V] [R : RepFunStore T K V] [OFE V] : {f : K → V // R.rep f} -n> T where
+  f x := ofFun x
+  ne.1 {_ _ _} H k := by rw [get_ofFun, get_ofFun]; exact H k
 
-@[simp] def StoreO.get [StoreLike T K V] (k : K) : StoreO T → V :=
-  fun s => StoreLike.get s.1 k
-
--- TODO: A `Proper` class could avoid the variable reordering.
-instance Store.get_ne [StoreLike T K V] [OFE V] (k : K) : NonExpansive (StoreO.get k : StoreO T → V) where
+instance get_ne [Store T K V] [OFE V] (k : K) : NonExpansive (Store.get · k : T → V) where
   ne {_ _ _} Ht := Ht k
 
-@[simp] def StoreO.set [StoreLike T K V] [OFE V] (k : K) : V → StoreO T → StoreO T :=
-  fun v s => StoreO.mk (StoreLike.set s.1 k v)
-
-@[simp] def StoreO.Equiv [StoreLike T K V] : StoreO T → StoreO T → Prop :=
-  (Store.Equiv ·.1 ·.1)
-
-instance StoreO.Equiv_trans [StoreLike T K V] : Trans (StoreO.Equiv : StoreO T → StoreO T → Prop) (StoreO.Equiv : StoreO T → StoreO T → Prop) (StoreO.Equiv : StoreO T → StoreO T → Prop) where
-  trans := by simp_all [Store.Equiv]
-
--- TODO: A `Proper` class could avoid the variable reordering.
-instance [Store T K V] [OFE V] (k : K) : NonExpansive₂ (StoreO.set k : V → StoreO T → StoreO T) where
+instance [Store T K V] [OFE V] (k : K) : NonExpansive₂ (Store.set · k · : T → V → T) where
   ne {n v1 v2} Hv {t1 t2} Ht k' := by
-    simp only [StoreO.set]
     cases (Classical.em (k = k'))
-    · rename_i H; rw [Store.get_set_eq H, Store.get_set_eq H]; exact Hv
-    · rename_i H; rw [Store.get_set_ne H, Store.get_set_ne H]; exact Ht k'
-
-@[simp] def StoreO.merge [StoreLike T K V] (op : V → V → V) (s1 s2 : StoreO T) : StoreO T :=
-  .mk (StoreLike.merge op s1.1 s2.1)
+    · rename_i H; rw [Store.get_set_eq H, Store.get_set_eq H]; exact Ht
+    · rename_i H; rw [Store.get_set_ne H, Store.get_set_ne H]; exact Hv k'
 
 instance [Store T K V] [OFE V] (op : V → V → V) [NonExpansive₂ op] :
-    NonExpansive₂ (StoreO.merge (T := T) op) where
-  ne n {_ _} Ht {_ _} Hs k := by
-    simp only [StoreO.merge, Store.get_merge]
-    exact NonExpansive₂.ne (Ht k) (Hs k)
+    NonExpansive₂ (Store.merge (T := T) op) where
+  ne n {_ _} Ht {_ _} Hs k := by simp only [Store.get_merge]; exact NonExpansive₂.ne (Ht k) (Hs k)
 
-@[simp] def StoreO.map [StoreLike T1 K V1] [Store T2 K V2] (f : V1 → V2) : StoreO T1 → StoreO T2 :=
-  fun t => ⟨StoreLike.map t.1 f⟩
+instance [Store T1 K V1] [Store T2 K V2] [OFE V1] [OFE V2] (f : K → V1 → V2) [∀ k, NonExpansive (f k)] [HasStoreMap T1 T2 K V1 V2] :
+    NonExpansive (dmap f : T1 → T2) where
+  ne _ {_ _} H k := by simp only [get_dmap]; exact NonExpansive.ne (H k)
 
-instance [StoreLike T1 K V1] [Store T2 K V2] [OFE V1] [OFE V2] (f : V1 → V2) [NonExpansive f] :
-    NonExpansive (StoreO.map f : StoreO T1 → StoreO T2) where
-  ne n {_ _} H k := by simp [StoreO.map, Store.get_map]; exact NonExpansive.ne (H k)
-
-instance StoreO_COFE [Store T K V] [COFE V] : COFE (StoreO T) where
-  compl c := ⟨StoreLike.ofFun <| COFE.compl <| c.map StoreO.toMap⟩
-  conv_compl {n c} k := by
-    rw [Store.ofFun_get]
-    exact COFE.conv_compl (c := Chain.map StoreO.toMap c) k
-
-@[simp] def StoreO.all [StoreLike T K V] (P : K → V → Prop) : StoreO T → Prop :=
-  fun t => StoreLike.all P t.1
-
-@[simp] def StoreO.dom [HeapLike T K V] : StoreO T → K → Prop :=
-  fun t k => HeapLike.dom t.1 k
-
-abbrev StoreO.union_F : Option V → Option V → Option V
-| .some v1 => fun _ => v1
-| .none => id
-
-@[simp] def StoreO.union [HeapLike T K V] (t1 t2 : StoreO T) : StoreO T :=
-  let F : Option V → Option V → Option V
-  | .some v1 => fun _ => v1
-  | .none => id
-  StoreO.merge F t1 t2
-
-@[simp] def StoreO.empty [HeapLike T K V] : StoreO T := ⟨HeapLike.empty⟩
-
-@[simp] def StoreO.delete [HeapLike T K V] : StoreO T → K → StoreO T :=
-  fun t k => .mk <| HeapLike.delete t.1 k
-
-@[simp] def StoreO.singleton [WithPoints T K V]: K → V → StoreO T :=
-  fun t k => ⟨WithPoints.point t k⟩
+instance Store_COFE [Store T K V] [HasStoreMap T T K V V] [COFE V] : COFE T where
+  compl c := HasStoreMap.dmap (fun k _ => COFE.compl <| c.map ⟨(Store.get · k), get_ne k⟩) (c 0)
+  conv_compl _ := by rw [get_dmap]; apply IsCOFE.conv_compl
 
 /- [3] -> [2] -/
-theorem StoreO.Equiv_of_eq [Store T K V] {t1 t2 : StoreO T} (H : t1 = t2) :
-  StoreO.Equiv t1 t2 := H▸rfl
+theorem Store.Equiv_of_eq [Store T K V] {t1 t2 : T} (H : t1 = t2) : Store.Equiv t1 t2 := H▸rfl
 
 /- [2] -> [1] -/
-theorem StoreO.Eqv_of_Equiv [Store T K V] [OFE V] {t1 t2 : StoreO T} (H : StoreO.Equiv t1 t2) :
+theorem Store.Eqv_of_Equiv [Store T K V] [OFE V] {t1 t2 : T} (H : Store.Equiv t1 t2) :
     t1 ≡ t2 := fun i => Equiv.of_eq <| congrFun H i
 
-/-- When the type is a StoreIso, equality coincides with pointwise equality ([2] -> [3]). -/
-theorem IsStoreIso.eq_of_Equiv [Store T K V] [IsStoreIso T K V] {t1 t2 : StoreO T} :
-    StoreO.Equiv t1 t2 → t1 = t2 :=
-  (StoreO.ext <| store_eq_of_Equiv ·)
+-- TODO: Delete me after refactor is complete
+theorem IsStoreIso.eq_of_Equiv [Store T K V] [IsoFunStore T K V] {t1 t2 : T} :
+    Store.Equiv t1 t2 → t1 = t2 := (store_eq_of_Equiv ·)
 
 /-- When the value is Leibniz, pointwise equality coincides with OFE equivalence. ([1] -> [2]), -/
-theorem IsStore.StoreO_Equiv_iff_leibniz [Store T K V] [OFE V] [Leibniz V] {t1 t2 : StoreO T}
-    (H : t1 ≡ t2) : StoreO.Equiv t1 t2 := funext ((forall_congr fun _ => propext leibniz).mp H ·)
+theorem IsStore.StoreO_Equiv_iff_leibniz [Store T K V] [OFE V] [Leibniz V] {t1 t2 : T}
+    (H : t1 ≡ t2) : Store.Equiv t1 t2 := funext ((forall_congr fun _ => propext leibniz).mp H ·)
 
-/-- When store is a StoreIso with Leibniz values, it is Leibniz -/
-instance [Store T K V] [IsStoreIso T K V] [COFE V] [Leibniz V] : Leibniz (StoreO T) where
-  eq_of_eqv {x y} H := by
-    apply StoreO.ext
-    rewrite [← IsStoreIso.get_ofFun x.car, ← IsStoreIso.get_ofFun y.car]
-    congr 1
-    apply funext
-    intro k
-    apply eq_of_eqv (H k)
+/-- When store is a StoreIso with Leibniz values, it is Leibniz ([1] → [3]) -/
+instance [Store T K V] [IsoFunStore T K V] [COFE V] [Leibniz V] : Leibniz T where
+  eq_of_eqv := IsStoreIso.store_eq_of_Equiv ∘ IsStore.StoreO_Equiv_iff_leibniz
 
-instance [Store T K V] [COFE V] [Discrete V] : Discrete (StoreO T) where
+instance [Store T K V] [COFE V] [Discrete V] : Discrete T where
   discrete_0 H k := discrete_0 <| H k
 
 end ofe
@@ -245,15 +204,15 @@ open CMRA
 
 /- ## A CMRA on Heaps -/
 
-variable [Heap T K V] [CMRA V]
+variable [Heap T K] [CMRA V]
 
-abbrev op_merge : Option V → Option V → Option V
+abbrev op_merge [CMRA V] : Option V → Option V → Option V
 | .some v1, .some v2 => Option.some (v1 • v2)
 | .some v1, .none    => Option.some v1
 | .none,    .some v2 => Option.some v2
 | _,        _        => Option.none
 
-instance : OFE.NonExpansive₂ (op_merge (V := V)) where
+instance [CMRA V] : OFE.NonExpansive₂ (op_merge (V := V)) where
   ne _ x1 x2 Hx y1 y2 Hy := by
     revert Hx Hy
     rcases x1 <;> rcases x2 <;> rcases y1 <;> rcases y2 <;> simp
@@ -267,159 +226,161 @@ theorem op_merge_comm {x y : Option V} : op_merge x y ≡ op_merge y x := by
   cases x <;> cases y <;> simp [op_merge]
   exact comm
 
-abbrev pcore_F : Option V → Option V
+abbrev pcore_F [CMRA V] : Option V → Option V
 | Option.some v => CMRA.pcore v
 | Option.none => Option.none
 
-instance : OFE.NonExpansive (pcore_F (V := V)) where
+instance [CMRA V] : OFE.NonExpansive (pcore_F (V := V)) where
   ne _ x1 x2 := by
     cases x1 <;> cases x2 <;> simp [pcore_F]
     exact (OFE.NonExpansive.ne ·)
 
-abbrev store_op (s1 s2 : StoreO T) : StoreO T := StoreO.merge op_merge s1 s2
-abbrev store_unit : StoreO T := StoreO.empty
-abbrev store_pcore (s : StoreO T) : Option (StoreO T) := some <| StoreO.map pcore_F s
-abbrev store_valid (s : StoreO T) : Prop := ∀ k, ✓ (StoreO.get k s : Option V)
-abbrev store_validN (n : Nat) (s : StoreO T) : Prop := ∀ k, ✓{n} (StoreO.get k s : Option V)
+abbrev store_op (s1 s2 : T V) : T V :=
+  Store.merge (K := K) (op_merge) s1 s2
+abbrev store_unit : T V := Heap.empty V
+abbrev store_pcore (s : T V) : Option (T V) := some <| HasStoreMap.map pcore_F s
+abbrev store_valid (s : T V) : Prop := ∀ k, ✓ (Store.get s k : Option V)
+abbrev store_validN (n : Nat) (s : T V) : Prop := ∀ k, ✓{n} (Store.get s k : Option V)
 
-theorem lookup_includedN n (m1 m2 : StoreO T) :
-  (∃ (z : StoreO T), m2 ≡{n}≡ store_op m1 z) ↔
-  ∀ i, (∃ z, (StoreO.get i m2) ≡{n}≡ (StoreO.get i m1) • z) := by
+theorem lookup_includedN n (m1 m2 : T V) :
+  (∃ (z : T V), m2 ≡{n}≡ store_op m1 z) ↔
+  ∀ i, (∃ z, (Store.get m2 i) ≡{n}≡ (Store.get m1 i) • z) := by
   constructor
   · intros H i
-    rcases H with ⟨⟨z⟩, Hz⟩
-    exists (StoreO.get i ⟨z⟩)
-    rcases m1 with ⟨m1⟩
-    rcases m2 with ⟨m2⟩
+    rcases H with ⟨z, Hz⟩
+    exists (Store.get z i)
+    sorry
+    -- simp_all [CMRA.op, optionOp]
+    -- have Hz' := Hz i
+    -- simp [Store.get_merge, op_merge] at Hz'
+    -- generalize HX : Store.get m1 i = X
+    -- generalize HZ : Store.get z i = Z
+    -- rw [HX, HZ] at Hz'
+    -- cases X <;> cases Z <;> simp_all
+  · intro H
+    rcases (Classical.axiomOfChoice H) with ⟨f, Hf⟩
+    -- apply Classical.not_forall_not.mp
+    -- intro HK
+    sorry  -- Trying to do this without ofFun
+    -- exists ⟨StoreLike.ofFun f⟩
+    -- intro i
+    -- apply (Hf i).trans
+    -- simp [store_op, Store.get_merge, op_merge, Store.ofFun_get]
+    -- generalize HX : StoreLike.get m1.car i = X
+    -- generalize HY : f i = Y
+    -- cases X <;> cases Y <;> simp_all [CMRA.op, optionOp]
+
+theorem lookup_included {m1 m2 : T V} :
+  (∃ (z : T V), m2 ≡ store_op m1 z) ↔
+  ∀ i, (∃ z, (Store.get m2 i) ≡ (Store.get m1 i) • z) := by
+  constructor
+  · intros H i
+    rcases H with ⟨z, Hz⟩
+    exists (Store.get z i)
     simp_all [CMRA.op, optionOp]
     have Hz' := Hz i
     simp [Store.get_merge, op_merge] at Hz'
-    generalize HX : StoreLike.get m1 i = X
-    generalize HZ : StoreLike.get z i = Z
+    generalize HX : get m1 i = X
+    generalize HZ : get z i = Z
     rw [HX, HZ] at Hz'
     cases X <;> cases Z <;> simp_all
   · intro H
     rcases (Classical.axiomOfChoice H) with ⟨f, Hf⟩
-    exists ⟨StoreLike.ofFun f⟩
-    intro i
-    apply (Hf i).trans
-    simp [store_op, Store.get_merge, op_merge, Store.ofFun_get]
-    generalize HX : StoreLike.get m1.car i = X
-    generalize HY : f i = Y
-    cases X <;> cases Y <;> simp_all [CMRA.op, optionOp]
+    sorry
+    -- exists ⟨StoreLike.ofFun f⟩
+    -- intro i
+    -- apply (Hf i).trans
+    -- simp [store_op, Store.get_merge, op_merge, Store.ofFun_get]
+    -- generalize HX : StoreLike.get m1.car i = X
+    -- generalize HY : f i = Y
+    -- cases X <;> cases Y <;> simp_all [CMRA.op, optionOp]
 
-theorem lookup_included {m1 m2 : StoreO T} :
-  (∃ (z : StoreO T), m2 ≡ store_op m1 z) ↔
-  ∀ i, (∃ z, (StoreO.get i m2) ≡ (StoreO.get i m1) • z) := by
-  constructor
-  · intros H i
-    rcases H with ⟨⟨z⟩, Hz⟩
-    exists (StoreO.get i ⟨z⟩)
-    rcases m1 with ⟨m1⟩
-    rcases m2 with ⟨m2⟩
-    simp_all [CMRA.op, optionOp]
-    have Hz' := Hz i
-    simp [Store.get_merge, op_merge] at Hz'
-    generalize HX : StoreLike.get m1 i = X
-    generalize HZ : StoreLike.get z i = Z
-    rw [HX, HZ] at Hz'
-    cases X <;> cases Z <;> simp_all
-  · intro H
-    rcases (Classical.axiomOfChoice H) with ⟨f, Hf⟩
-    exists ⟨StoreLike.ofFun f⟩
-    intro i
-    apply (Hf i).trans
-    simp [store_op, Store.get_merge, op_merge, Store.ofFun_get]
-    generalize HX : StoreLike.get m1.car i = X
-    generalize HY : f i = Y
-    cases X <;> cases Y <;> simp_all [CMRA.op, optionOp]
-
-instance StoreO_CMRA : CMRA (StoreO T) where
+instance StoreO_CMRA : CMRA (T V) where
   pcore := store_pcore
   op := store_op
   ValidN := store_validN
   Valid := store_valid
   op_ne := ⟨fun _ _ _ H => OFE.NonExpansive₂.ne .rfl H⟩
   pcore_ne {n x y cx} H := by
-    simp only [store_pcore, StoreO.map, Option.some.injEq, exists_eq_left']
+    simp only [store_pcore, Option.some.injEq, exists_eq_left']
     refine (· ▸ fun k => ?_)
-    simp only [Store.get_map]
+    simp only [get_dmap]
     exact OFE.NonExpansive.ne (H k)
-  validN_ne Hx H k := CMRA.validN_ne (OFE.NonExpansive.ne Hx) (H k)
+  validN_ne Hx H k := CMRA.validN_ne (OFE.NonExpansive.ne (f := (Store.get · k : T V → Option V)) Hx) (H k)
   valid_iff_validN {x} :=
     ⟨fun H n k => valid_iff_validN.mp (H k) n, fun H k => valid_iff_validN.mpr (H · k)⟩
   validN_succ H k := validN_succ (H k)
   validN_op_left {n x1 x2} H k := by
-    apply CMRA.validN_op_left (y := StoreO.get k x2)
+    apply CMRA.validN_op_left (y := Store.get x2 k)
     simp [CMRA.op, optionOp, store_validN, Store.get_merge, op_merge] at ⊢ H
     have H' := H k
-    generalize HX : StoreLike.get x1.car k = X
-    generalize HY : StoreLike.get x2.car k = Y
+    generalize HX : Store.get x1 k = X
+    generalize HY : Store.get x2 k = Y
     simp_all
-    cases X <;> cases Y <;> simp_all
+    cases X <;> cases Y <;> simp_all [CMRA.op, optionOp]
+    all_goals sorry
   assoc := by
-    rintro ⟨x⟩ ⟨y⟩ ⟨z⟩ k
+    rintro x y z k
     simp [store_op, Store.get_merge]
     exact op_merge_assoc
   comm := by
-    rintro ⟨x⟩ ⟨y⟩ k
+    rintro x y k
     simp [store_op, Store.get_merge]
     exact op_merge_comm
   pcore_op_left {x cx} := by
     refine (fun H => ?_)
     have H' : store_op ((store_pcore x).getD x) x ≡ x := by
-      rcases cx with ⟨cx⟩
       intro k
       simp [store_op, store_pcore, store_op]
-      rw [Store.get_merge]
-      simp [store_pcore] at H
-      simp [op_merge, Store.get_map]
-      unfold pcore_F
-      generalize HX : StoreLike.get x.car k = X
-      cases X <;> simp
-      rename_i v
-      generalize HY : pcore v = Y
-      cases Y <;> simp
-      exact pcore_op_left HY
+      sorry
+      -- rw [Store.get_merge (T := T V)]
+      -- simp [store_pcore] at H
+      -- simp [op_merge, get_dmap]
+      -- unfold pcore_F
+      -- generalize HX : StoreLike.get x.car k = X
+      -- cases X <;> simp
+      -- rename_i v
+      -- generalize HY : pcore v = Y
+      -- cases Y <;> simp
+      -- exact pcore_op_left HY
     apply (H ▸ H')
   pcore_idem {x cx} := by
     refine (fun H => ?_)
     have H' : ((store_pcore ((store_pcore x).getD x)).getD ((store_pcore x).getD x)) ≡ ((store_pcore x).getD x) := by
       intro k
       rw [H]
-      simp only [Option.getD_some, StoreO.map]
-      rw [Store.get_map]
-      simp [store_pcore] at H
-      rw [← H]
-      simp [pcore_F, Store.get_map]
-      generalize HX : StoreLike.get x.car k = X
-      cases X <;> simp
-      rename_i v
-      generalize HY : pcore v = Y
-      cases Y <;> simp
-      exact pcore_idem HY
+      sorry
+      -- simp only [Option.getD_some, StoreO.map]
+      -- rw [Store.get_map]
+      -- simp [store_pcore] at H
+      -- rw [← H]
+      -- simp [pcore_F, Store.get_map]
+      -- generalize HX : StoreLike.get x.car k = X
+      -- cases X <;> simp
+      -- rename_i v
+      -- generalize HY : pcore v = Y
+      -- cases Y <;> simp
+      -- exact pcore_idem HY
     apply (H ▸ H')
   pcore_op_mono := by
     apply pcore_op_mono_of_core_op_mono
-    let core' (x : StoreO T) := (store_pcore x).getD x
-    let le' (x y : StoreO T) := ∃ z, y ≡ store_op x z
+    let core' (x : T V) := (store_pcore x).getD x
+    let le' (x y : T V) := ∃ z, y ≡ store_op x z
 
     -- First direction, no countability used
-    have Hcore'le'1 (x y : StoreO T) : le' x y → ∀ (i : K), (StoreO.get i x ≼ StoreO.get i y) := by
+    have Hcore'le'1 (x y : T V) : le' x y → ∀ (i : K), (Store.get x i ≼ Store.get y i) := by
       intros H i
-      rcases H with ⟨⟨z⟩, Hz⟩
-      exists (StoreO.get i ⟨z⟩)
-      rcases x with ⟨x⟩
-      rcases y with ⟨y⟩
+      rcases H with ⟨z, Hz⟩
+      exists (Store.get z i)
       simp_all [CMRA.op, optionOp]
       have Hz' := Hz i
       simp [Store.get_merge, op_merge] at Hz'
-      generalize HX : StoreLike.get x i = X
-      generalize HZ : StoreLike.get z i = Z
+      generalize HX : Store.get x i = X
+      generalize HZ : Store.get z i = Z
       rw [HX, HZ] at Hz'
       cases X <;> cases Z <;> simp_all
 
-    suffices ∀ x y : StoreO T, le' x y → le' (core' x) (core' y) by
+    suffices ∀ x y : T V, le' x y → le' (core' x) (core' y) by
       rintro x cx y Hxy' Hx
       have Hxy := this x y Hxy'
       unfold core' at Hxy
@@ -430,155 +391,159 @@ instance StoreO_CMRA : CMRA (StoreO T) where
     unfold le'
     refine lookup_included.mpr ?_
     intro i
-    suffices (core (StoreO.get i x)) ≼ (core (StoreO.get i y)) by
-      simp_all [core', pcore_F, core, Store.get_map]
+    suffices (core (Store.get x i)) ≼ (core (Store.get y i)) by
+      simp_all [core', pcore_F, core, get_dmap]
       split <;> split <;> simp_all [pcore, optionCore, this] <;> exact this
     exact core_mono (Hcore'le'1 x y H' i)
 
   extend := by
     intro n m y1 y2 Hm Heq
-    have F (i : K) := @CMRA.extend (Option V) _ n (StoreO.get i m) (StoreO.get i y1) (StoreO.get i y2) (Hm i) ?G
+    have F (i : K) := @CMRA.extend (Option V) _ n (Store.get m i) (Store.get y1 i) (Store.get y2 i) (Hm i) ?G
     case G =>
-      apply ((Store.get_ne i).ne Heq).trans
-      simp [CMRA.op, optionOp]
-      rw [Store.get_merge]
-      simp [op_merge]
-      generalize HX : StoreLike.get y1.car i = X
-      generalize HY : StoreLike.get y2.car i = Y
-      cases X <;> cases Y <;> simp
-    exists ⟨StoreLike.ofFun (F · |>.fst)⟩
-    exists ⟨StoreLike.ofFun (F · |>.snd.fst)⟩
-    refine ⟨fun i => ?_, fun i => ?_, fun i => ?_⟩
-      <;> simp [store_op, Store.get_merge, Store.ofFun_get]
-      <;> rcases (F i) with ⟨z1, z2, Hm, Hz1, Hz2⟩
-    · refine Hm.trans ?_
-      simp [CMRA.op, op_merge, optionOp]
-      cases z1 <;> cases z2 <;> simp
-    · exact Hz1
-    · exact Hz2
+      -- apply ((Store.get_ne i).ne Heq).trans
+      -- simp [CMRA.op, optionOp]
+      -- rw [Store.get_merge]
+      -- simp [op_merge]
+      -- generalize HX : StoreLike.get y1.car i = X
+      -- generalize HY : StoreLike.get y2.car i = Y
+      -- cases X <;> cases Y <;> simp
+      sorry
+    sorry
+    -- exists ⟨StoreLike.ofFun (F · |>.fst)⟩
+    -- exists ⟨StoreLike.ofFun (F · |>.snd.fst)⟩
+    -- refine ⟨fun i => ?_, fun i => ?_, fun i => ?_⟩
+    --   <;> simp [store_op, Store.get_merge, Store.ofFun_get]
+    --   <;> rcases (F i) with ⟨z1, z2, Hm, Hz1, Hz2⟩
+    -- · refine Hm.trans ?_
+    --   simp [CMRA.op, op_merge, optionOp]
+    --   cases z1 <;> cases z2 <;> simp
+    -- · exact Hz1
+    -- · exact Hz2
 
-instance StoreO_UCMRA : UCMRA (StoreO T) where
+instance StoreO_UCMRA : UCMRA (T V) where
   unit := store_unit
-  unit_valid := by simp [CMRA.Valid, store_valid, optionValid, HeapLike.empty, Store.ofFun_get]
+  unit_valid := by simp [CMRA.Valid, store_valid, optionValid, store_unit, Heap.get_empty]
   unit_left_id := by
     intro x k
-    simp [CMRA.op, op_merge, HeapLike.empty, Store.get_merge, Store.ofFun_get]
-    generalize HX : StoreLike.get x.car k = X <;> cases X <;> simp
-  pcore_unit k := by simp [CMRA.pcore, Store.get_map, pcore_F, HeapLike.empty, Store.ofFun_get]
+    simp [CMRA.op, op_merge, Store.get_merge, store_unit, Heap.get_empty]
+    generalize HX : Store.get x k = X <;> cases X <;> simp
+  pcore_unit := by intro k; simp [CMRA.pcore, get_dmap, pcore_F, store_unit, Heap.get_empty]
 end cmra
 
 section heap_laws
 
-variable {T K V : Type _} [Heap T K V] [CMRA V]
+variable {K V : Type _} [Heap T K] [CMRA V]
 open CMRA
 
 
-theorem lookup_validN_Some {m : StoreO T} : ✓{n} m → StoreO.get i m ≡{n}≡ some x → ✓{n} x := by
-  suffices ✓{n} StoreO.get i m → StoreO.get i m ≡{n}≡ some x → ✓{n} x by
+theorem lookup_validN_Some {m : T V} : ✓{n} m → Store.get m i ≡{n}≡ some x → ✓{n} x := by
+  suffices ✓{n} Store.get m i → Store.get m i ≡{n}≡ some x → ✓{n} x by
     exact fun Hv => (this (Hv i) ·)
   simp only [ValidN, optionValidN]
   split <;> rename_i He <;> rw [He]
   · exact fun Hv => (·.validN |>.mp Hv)
   · rintro _ ⟨⟩
 
-theorem lookup_valid_Some {m : StoreO T} (Hv : ✓ m) (He : StoreO.get i m ≡ some x) : ✓ x :=
+theorem lookup_valid_Some {m : T V} (Hv : ✓ m) (He : Store.get m i ≡ some x) : ✓ x :=
   valid_iff_validN.mpr (fun _ => lookup_validN_Some Hv.validN He.dist)
 
-theorem insert_validN {m : StoreO T} (Hx : ✓{n} x) (Hm : ✓{n} m) : ✓{n} (StoreO.set i x m) := by
+theorem insert_validN {m : T V} (Hx : ✓{n} x) (Hm : ✓{n} m) : ✓{n} (Store.set m i x) := by
   intro k
-  simp [CMRA.Valid]
+  simp [CMRA.ValidN]
   if He : i = k
-    then rw [Heap.get_set_eq He]; exact Hx
-    else rw [Heap.get_set_ne (He ·)]; exact Hm k
+    then rw [get_set_eq (T := T V) He]; exact Hx
+    else rw [get_set_ne (T := T V) (He ·)]; apply Hm
 
-theorem insert_valid {m : StoreO T} (Hx : ✓ x) (Hm : ✓ m) : ✓ (StoreO.set i x m) :=
+theorem insert_valid {m : T V} (Hx : ✓ x) (Hm : ✓ m) : ✓ (Store.set m i x) :=
   valid_iff_validN.mpr (fun _ => insert_validN Hx.validN Hm.validN)
 
-theorem singleton_valid : ✓ (StoreO.singleton i x : StoreO T) ↔ ✓ x := by
-  simp only [StoreO.singleton, StoreO.get]
+theorem point_valid : ✓ (Heap.point i x : T V) ↔ ✓ x := by
+  simp only [Heap.point, Store.get]
   constructor <;> intro H
-  · have H' := H i; simp [Heap.point_get_eq rfl] at H'; exact H'
+  · have H' := H i; simp [Heap.point_get_eq rfl] at H'; rw [get_set_eq (T := T V) rfl] at H'; exact H'
   · intro k
     if He : i = k
-      then simp [StoreO.get]; rw [Heap.point_get_eq He]; trivial
-      else simp [StoreO.get]; rw [Heap.point_get_ne He]; trivial
+      then rw [get_set_eq (T := T V) He]; trivial
+      else rw [get_set_ne (T := T V) He, Heap.get_empty]; trivial
 
-theorem delete_validN {m : StoreO T} (Hv : ✓{n} m) : ✓{n} (StoreO.delete m i) := by
+theorem delete_validN {m : T V} (Hv : ✓{n} m) : ✓{n} (Heap.delete m i) := by
   intro k
   if He : i = k
-    then simp only [StoreO.get, StoreO.delete]; rw [Store.get_set_eq He]; trivial
-    else simp only [StoreO.get, StoreO.delete]; rw [Store.get_set_ne He]; exact Hv k
+    then simp only [Heap.delete]; rw [Store.get_set_eq (T := T V) He]; trivial
+    else simp only [Heap.delete]; rw [Store.get_set_ne (T := T V) He]; exact Hv k
 
-theorem delete_valid {m : StoreO T} (Hv : ✓ m) : ✓ (StoreO.delete m i) :=
+theorem delete_valid {m : T V} (Hv : ✓ m) : ✓ (Heap.delete m i) :=
   valid_iff_validN.mpr (fun _ => delete_validN Hv.validN)
 
-theorem insert_singleton_op {m : StoreO T} (Hemp : StoreO.get i m = none) :
-    StoreO.Equiv (StoreO.set i x m) (StoreO.singleton i x • m) := by
-  simp_all [StoreO.singleton, StoreO.set, CMRA.op, op, StoreLike.merge, op_merge, Store.Equiv]
+theorem insert_point_op {m : T V} (Hemp : Store.get m i = none) :
+    Store.Equiv (Store.set m i x) (Heap.point i x • m) := by
+  simp_all [CMRA.op, op, op_merge, Store.Equiv]
   refine funext (fun k => ?_)
   if He : i = k
     then
-      rw [Store.get_set_eq He, Heap.ofFun_get, Heap.point_get_eq He, He.symm, Hemp]
-      split
-      · rename_i Hk; rcases Hk
-      · rfl
-      · rename_i Hk; rcases Hk
-      · (expose_names; exact Option.eq_none_iff_forall_ne_some.mpr fun a a_1 => h_1 a a_1 rfl)
+      sorry
+      -- rw [Store.get_set_eq (T := T V) He, store_op, get_merge, Heap.point_get_eq He, He.symm, Hemp]
+      -- split
+      -- · rename_i Hk; rcases Hk
+      -- · rfl
+      -- · rename_i Hk; rcases Hk
+      -- · (expose_names; exact Option.eq_none_iff_forall_ne_some.mpr fun a a_1 => h_1 a a_1 rfl)
     else
-      rw [Store.get_set_ne He, Heap.ofFun_get, Heap.point_get_ne He]
-      split <;> rename_i Hk _
-      · rcases Hk
-      · rcases Hk
-      · trivial
-      · (expose_names; exact Option.eq_none_iff_forall_ne_some.mpr fun a => h_1 a rfl)
+      sorry
+      -- rw [Store.get_set_ne He, Heap.ofFun_get, Heap.point_get_ne He]
+      -- split <;> rename_i Hk _
+      -- · rcases Hk
+      -- · rcases Hk
+      -- · trivial
+      -- · (expose_names; exact Option.eq_none_iff_forall_ne_some.mpr fun a => h_1 a rfl)
 
-theorem insert_singleton_op_eq [IsStoreIso T K (Option V)] {m : StoreO T} (Hemp : StoreO.get i m = none) :
-    StoreO.set i x m = StoreO.singleton i x • m :=
-  IsStoreIso.eq_of_Equiv (insert_singleton_op Hemp)
+theorem insert_point_op_eq [IsoFunStore (T V) K (Option V)] {m : T V} (Hemp : Store.get m i = none) :
+    Store.set m i x = Heap.point i x • m :=
+  IsStoreIso.eq_of_Equiv (insert_point_op Hemp)
 
-theorem singleton_core {i : K} {x : V} {cx} (Hpcore : pcore x = some cx) :
-    StoreO.Equiv (core (StoreO.singleton i (some x) : StoreO T)) ((StoreO.singleton i (some cx) : StoreO T)) := by
+theorem point_core {i : K} {x : V} {cx} (Hpcore : pcore x = some cx) :
+    Store.Equiv (core (Heap.point i (some x) : T V)) ((Heap.point i (some cx) : T V)) := by
   simp [core, pcore]
   rw [← Hpcore]
-  unfold StoreLike.map
   unfold Store.Equiv
   apply funext
   intro k
   if He : i = k
-    then rw [Heap.ofFun_get, Heap.point_get_eq He, Heap.point_get_eq He]
-    else rw [Heap.ofFun_get, Heap.point_get_ne He, Heap.point_get_ne He]
+    then sorry  -- rw [Heap.ofFun_get, Heap.point_get_eq He, Heap.point_get_eq He]
+    else sorry  -- rw [Heap.ofFun_get, Heap.point_get_ne He, Heap.point_get_ne He]
 
-theorem singleton_core_eq [IsStoreIso T K (Option V)] {i : K} {x : V} {cx} (Hpcore : pcore x = some cx) :
-    core (StoreO.singleton i (some x) : StoreO T) = (StoreO.singleton i (some cx) : StoreO T) :=
-  IsStoreIso.eq_of_Equiv (singleton_core Hpcore)
+theorem point_core_eq [IsoFunStore (T V) K (Option V)] {i : K} {x : V} {cx} (Hpcore : pcore x = some cx) :
+    core (Heap.point i (some x) : T V) = (Heap.point i (some cx) : T V) :=
+  IsStoreIso.eq_of_Equiv (point_core Hpcore)
 
-theorem singleton_core' {i : K} {x : V} {cx} (Hpcore : pcore x ≡ some cx) :
-    core (StoreO.singleton i (some x)) ≡ (StoreO.singleton i (some cx) : StoreO T) := by
+theorem point_core' {i : K} {x : V} {cx} (Hpcore : pcore x ≡ some cx) :
+    core (Heap.point i (some x)) ≡ (Heap.point i (some cx) : T V) := by
   simp [core, pcore]
-  unfold StoreLike.map
   intro k
   if He : i = k
-    then rw [Heap.ofFun_get, Heap.point_get_eq He, Heap.point_get_eq He]; exact Hpcore
-    else rw [Heap.ofFun_get, Heap.point_get_ne He, Heap.point_get_ne He]
+    then sorry -- rw [Heap.ofFun_get, Heap.point_get_eq He, Heap.point_get_eq He]; exact Hpcore
+    else sorry -- rw [Heap.ofFun_get, Heap.point_get_ne He, Heap.point_get_ne He]
 
-theorem singleton_core_total [IsTotal V] {i : K} {x : V} :
-    StoreO.Equiv (core (StoreO.singleton i (some x) : StoreO T)) ((StoreO.singleton i (some (core x)))) := by
+theorem point_core_total [IsTotal V] {i : K} {x : V} :
+    Store.Equiv (core (Heap.point i (some x) : T V)) ((Heap.point i (some (core x)))) := by
   obtain ⟨xc, Hxc⟩ := total x
-  apply StoreO.Equiv_trans.trans (singleton_core Hxc)
-  simp [core, Hxc]
-  rfl
+  sorry
+  -- apply Equiv_trans.trans (point_core Hxc)
+  -- simp [core, Hxc]
+  -- rfl
 
-theorem singleton_core_total_eq [IsTotal V] [IsStoreIso T K (Option V)] {i : K} {x : V} :
-    core (StoreO.singleton i (some x) : StoreO T) = (StoreO.singleton i (some (core x))) :=
-  IsStoreIso.eq_of_Equiv singleton_core_total
+theorem point_core_total_eq [IsTotal V] [IsoFunStore (T V) K (Option V)] {i : K} {x : V} :
+    core (Heap.point i (some x) : T V) = (Heap.point i (some (core x))) :=
+  IsStoreIso.eq_of_Equiv point_core_total
 
-theorem singleton_op {i : K} {x y : V} :
-    StoreO.Equiv ((StoreO.singleton i (some x) : StoreO T) • (StoreO.singleton i (some y))) ((StoreO.singleton i (some (x • y)))) := by
-  unfold StoreO.Equiv
+theorem point_op {i : K} {x y : V} :
+    Store.Equiv ((Heap.point i (some x) : T V) • (Heap.point i (some y))) ((Heap.point i (some (x • y)))) := by
   unfold Store.Equiv
   apply funext
   intro k
   simp [op]
+  sorry
+  /-
   rw [Store.get_merge]
   unfold op_merge
   if He : i = k
@@ -592,28 +557,30 @@ theorem singleton_op {i : K} {x y : V} :
       rw [Heap.point_get_ne He]
       simp only []
       rw [Heap.point_get_ne He]
+  -/
 
-theorem singleton_op_eq [IsStoreIso T K (Option V)] {i : K} {x y : V} :
-    (StoreO.singleton i (some x) : StoreO T) • (StoreO.singleton i (some y)) = (StoreO.singleton i (some (x • y))) :=
-  IsStoreIso.eq_of_Equiv singleton_op
+theorem point_op_eq [IsoFunStore (T V) K (Option V)] {i : K} {x y : V} :
+    (Heap.point i (some x) : T V) • (Heap.point i (some y)) = (Heap.point i (some (x • y))) :=
+  IsStoreIso.eq_of_Equiv point_op
 
-theorem gmap_core_id {m : StoreO T} (H : ∀ i (x : V), (StoreO.get i m = some x) → CoreId x) : CoreId m := by
+theorem gmap_core_id {m : T V} (H : ∀ i (x : V), (Store.get m i = some x) → CoreId x) : CoreId m := by
   constructor
   intro i
-  simp [StoreO.map]
-  rw [Store.get_map]
-  simp [pcore_F]
-  split
-  · rename_i H'
-    rw [H']
-    exact (H _ _ H').core_id
-  · rename_i H'
-    rw [H']
+  sorry
+  -- rw [HasStoreMap.get_dmap]
+  -- simp [pcore_F]
+  -- split
+  -- · rename_i H'
+  --   rw [H']
+  --   exact (H _ _ H').core_id
+  -- · rename_i H'
+  --   rw [H']
 
-instance gmap_core_id' {m : StoreO T} (H : ∀ x : V, CoreId x) : CoreId m := by
+instance gmap_core_id' {m : T V} (H : ∀ x : V, CoreId x) : CoreId m := by
   constructor
   intro i
-  simp [StoreO.map]
+  sorry
+  /-
   rw [Store.get_map]
   simp [pcore_F]
   split
@@ -622,10 +589,13 @@ instance gmap_core_id' {m : StoreO T} (H : ∀ x : V, CoreId x) : CoreId m := by
     apply (H _).core_id
   · rename_i H'
     rw [H']
+  -/
 
-instance gmap_singleton_core_id (H : CoreId (x : V)) : CoreId (StoreO.singleton i (some x) : StoreO T) := by
+instance gmap_point_core_id (H : CoreId (x : V)) : CoreId (Heap.point i (some x) : T V) := by
   constructor
   intro k
+  sorry
+  /-
   simp [Store.get_map]
   if He : i = k
     then
@@ -634,14 +604,17 @@ instance gmap_singleton_core_id (H : CoreId (x : V)) : CoreId (StoreO.singleton 
       exact H.core_id
     else
       rw [Heap.point_get_ne He]
+    -/
 
-theorem singleton_includedN_l {m : StoreO T} :
-    (StoreO.singleton i (some x) : StoreO T) ≼{n} m ↔ ∃ y, (StoreO.get i m  ≡{n}≡ some y) ∧ some x ≼{n} some y := by
+theorem point_includedN_l {m : T V} :
+    (Heap.point i (some x) : T V) ≼{n} m ↔ ∃ y, (Store.get m i ≡{n}≡ some y) ∧ some x ≼{n} some y := by
   constructor
   · rintro ⟨z, Hz⟩
     have Hz' := Hz i
     simp [CMRA.op, op] at Hz'
-    rw [Store.get_merge] at Hz'
+    sorry
+    /-
+    rw [get_merge] at Hz'
     simp [op_merge] at Hz'
     rw [Heap.point_get_eq rfl] at Hz'
     generalize Hz0 : StoreLike.get z.car i = z0
@@ -651,91 +624,96 @@ theorem singleton_includedN_l {m : StoreO T} :
       exists (x • v)
       refine ⟨Hz', ?_⟩
       exists v
+    -/
   · rintro ⟨y, Hy, z, Hz⟩
-    exists StoreO.set i z m
+    exists Store.set m i z
     intro j
     if He : i = j
       then
-        simp [StoreO.singleton]
-        simp [StoreO.get, He] at Hy
-        refine Hy.trans (Hz.trans ?_)
-        simp [CMRA.op, Store.get_merge, Heap.point_get_eq He, Heap.get_set_eq He, op_merge, optionOp]
-        cases z <;> simp
+        sorry
+        -- simp [Heap.point]
+        -- simp [StoreO.get, He] at Hy
+        -- refine Hy.trans (Hz.trans ?_)
+        -- simp [CMRA.op, Store.get_merge, Heap.point_get_eq He, Heap.get_set_eq He, op_merge, optionOp]
+        -- cases z <;> simp
       else
-        simp [StoreO.singleton, CMRA.op]
-        rw [Store.get_merge, Heap.point_get_ne He, Heap.get_set_ne He]
-        simp [op_merge]
-        cases (StoreLike.get m.car j) <;> simp
+        sorry
+        -- simp [StoreO.point, CMRA.op]
+        -- rw [Store.get_merge, Heap.point_get_ne He, Heap.get_set_ne He]
+        -- simp [op_merge]
+        -- cases (StoreLike.get m.car j) <;> simp
 
-theorem singleton_included_l {m : StoreO T} :
-    (StoreO.singleton i (some x) : StoreO T) ≼ m ↔ ∃ y, (StoreO.get i m ≡ some y) ∧ some x ≼ some y := by
+theorem point_included_l {m : T V} :
+    (Heap.point i (some x) : T V) ≼ m ↔ ∃ y, (Store.get m i ≡ some y) ∧ some x ≼ some y := by
   constructor
   · rintro ⟨z, Hz⟩
     have Hz' := Hz i
     simp [CMRA.op, op] at Hz'
-    rw [Store.get_merge] at Hz'
-    simp [op_merge] at Hz'
-    rw [Heap.point_get_eq rfl] at Hz'
-    generalize Hz0 : StoreLike.get z.car i = z0
-    cases z0 <;> simp [Hz0] at Hz'
-    · exists x
-    · rename_i v
-      exists (x • v)
-      refine ⟨Hz', ?_⟩
-      exists v
+    sorry
+    -- rw [Store.get_merge] at Hz'
+    -- simp [op_merge] at Hz'
+    -- rw [Heap.point_get_eq rfl] at Hz'
+    -- generalize Hz0 : StoreLike.get z.car i = z0
+    -- cases z0 <;> simp [Hz0] at Hz'
+    -- · exists x
+    -- · rename_i v
+    --   exists (x • v)
+    --   refine ⟨Hz', ?_⟩
+    --   exists v
   · rintro ⟨y, Hy, z, Hz⟩
-    exists StoreO.set i z m
+    exists Store.set m i z
     intro j
     if He : i = j
       then
-        simp [StoreO.singleton]
-        simp [StoreO.get, He] at Hy
-        refine Hy.trans (Hz.trans ?_)
-        simp [CMRA.op, Store.get_merge, Heap.point_get_eq He, Heap.get_set_eq He, op_merge, optionOp]
-        cases z <;> simp
+        sorry
+        -- simp [StoreO.point]
+        -- simp [StoreO.get, He] at Hy
+        -- refine Hy.trans (Hz.trans ?_)
+        -- simp [CMRA.op, Store.get_merge, Heap.point_get_eq He, Heap.get_set_eq He, op_merge, optionOp]
+        -- cases z <;> simp
       else
-        simp [StoreO.singleton, CMRA.op]
-        rw [Store.get_merge, Heap.point_get_ne He, Heap.get_set_ne He]
-        simp [op_merge]
-        generalize Hx : StoreLike.get m.car j = x
-        cases x <;> simp
+        sorry
+        -- simp [StoreO.point, CMRA.op]
+        -- rw [Store.get_merge, Heap.point_get_ne He, Heap.get_set_ne He]
+        -- simp [op_merge]
+        -- generalize Hx : StoreLike.get m.car j = x
+        -- cases x <;> simp
 
-theorem singleton_included_exclusive_l {m : StoreO T} (He : Exclusive x) (Hv : ✓ m) :
-    (StoreO.singleton i (some x) : StoreO T) ≼ m ↔ (StoreO.get i m ≡ some x) := by
-  apply singleton_included_l.trans
+theorem point_included_exclusive_l {m : T V} (He : Exclusive x) (Hv : ✓ m) :
+    (Heap.point i (some x) : T V) ≼ m ↔ (Store.get m i ≡ some x) := by
+  apply point_included_l.trans
   constructor
   · rintro ⟨y, Hy, Hxy⟩
     suffices x ≡ y by apply Hy.trans this.symm
     exact some_inc_exclusive Hxy <| lookup_valid_Some Hv Hy
   · intro _; exists x
 
-theorem singleton_included :
-    (StoreO.singleton i (some x) : StoreO T) ≼ (StoreO.singleton i (some y)) ↔ some x ≼ some y := by
-  apply singleton_included_l.trans
+theorem point_included :
+    (Heap.point i (some x) : T V) ≼ (Heap.point i (some y)) ↔ some x ≼ some y := by
+  apply point_included_l.trans
   constructor
   · rintro ⟨z, Hz, Hxz⟩
-    simp [StoreO.get, StoreO.singleton] at Hz
     rw [Heap.point_get_eq rfl] at Hz
     exact inc_of_inc_of_eqv Hxz Hz.symm
   · intro H
     exists y
-    simp [StoreO.get, StoreO.singleton]
     rw [Heap.point_get_eq rfl]
     exact ⟨.rfl, H⟩
 
-theorem singleton_included_total [IsTotal V] :
-    (StoreO.singleton i (some x) : StoreO T) ≼ (StoreO.singleton i (some y))  ↔ x ≼ y :=
-  singleton_included.trans <| some_inc_total.trans <| Eq.to_iff rfl
+theorem point_included_total [IsTotal V] :
+    (Heap.point i (some x) : T V) ≼ (Heap.point i (some y))  ↔ x ≼ y :=
+  point_included.trans <| some_inc_total.trans <| Eq.to_iff rfl
 
-theorem singleton_included_mono (Hinc : x ≼ y) : (StoreO.singleton i (some x) : StoreO T) ≼ (StoreO.singleton i (some y)) :=
-  singleton_included.mpr <| some_inc.mpr <| .inr Hinc
+theorem point_included_mono (Hinc : x ≼ y) : (Heap.point i (some x) : T V) ≼ (Heap.point i (some y)) :=
+  point_included.mpr <| some_inc.mpr <| .inr Hinc
 
-instance singleton_cancelable (H : Cancelable (some x)) : Cancelable (StoreO.singleton i (some x) : StoreO T) := by
+instance point_cancelable (H : Cancelable (some x)) : Cancelable (Heap.point i (some x) : T V) := by
   constructor
   intro n m1 m2 Hv He j
   have Hv' := Hv j; clear Hv
   have He' := He j; clear He
-  simp_all [StoreO.singleton, CMRA.op, store_op, StoreO.merge, Store.get_merge]
+  /-
+  simp_all [StoreO.point, CMRA.op, store_op, StoreO.merge, Store.get_merge]
   if He : i = j
     then
       rw [Heap.point_get_eq He] at *
@@ -756,84 +734,84 @@ instance singleton_cancelable (H : Cancelable (some x)) : Cancelable (StoreO.sin
       rw [HX, HY] at He'
       rw [HX] at Hv'
       cases X <;> cases Y <;> simp_all [op_merge, CMRA.op, optionOp]
+  -/
+  sorry
 
-instance heap_cancelable {m : StoreO T} [Hid : ∀ x : V, IdFree x] [Hc : ∀ x : V, Cancelable x] : Cancelable m := by
+instance heap_cancelable {m : T V} [Hid : ∀ x : V, IdFree x] [Hc : ∀ x : V, Cancelable x] : Cancelable m := by
   constructor
   intro n m1 m2 Hv He i
-  apply CMRA.cancelableN (x := StoreLike.get m.car i)
+  apply CMRA.cancelableN (x := Store.get m i)
   · have Hv' := Hv i
-    simp [StoreO.get, CMRA.op, op] at Hv'
-    rw [Store.get_merge] at Hv'
-    generalize HX : (StoreLike.get m.car i) = X
-    generalize HY : (StoreLike.get m1.car i) = Y
-    simp_all [CMRA.op, op, op_merge, optionOp]
-    cases X <;> cases Y <;> simp_all
+    simp [CMRA.op, op] at Hv'
+    sorry
+    -- rw [Store.get_merge] at Hv'
+    -- generalize HX : (StoreLike.get m.car i) = X
+    -- generalize HY : (StoreLike.get m1.car i) = Y
+    -- simp_all [CMRA.op, op, op_merge, optionOp]
+    -- cases X <;> cases Y <;> simp_all
   · have He' := He i
     simp_all [CMRA.op, op, optionOp]
-    rw [Store.get_merge] at He'
-    simp [op_merge] at He'
-    generalize HX : (StoreLike.get m.car i) = X
-    generalize HY : (StoreLike.get m1.car i) = Y
-    generalize HZ : (StoreLike.get m2.car i) = Z
-    rw [HX, HY] at He'
-    cases X <;> cases Y <;> cases Z <;> simp_all [Store.get_merge, op_merge]
+    sorry
+    -- rw [Store.get_merge] at He'
+    -- simp [op_merge] at He'
+    -- generalize HX : (StoreLike.get m.car i) = X
+    -- generalize HY : (StoreLike.get m1.car i) = Y
+    -- generalize HZ : (StoreLike.get m2.car i) = Z
+    -- rw [HX, HY] at He'
+    -- cases X <;> cases Y <;> cases Z <;> simp_all [Store.get_merge, op_merge]
 
-theorem insert_op {m1 m2 : StoreO T} :
-    StoreO.Equiv ((StoreO.set i (x • y) (m1 • m2))) ((StoreO.set i x m1) • (StoreO.set i y m2)) := by
-  simp [StoreO.Equiv, Store.Equiv]
+theorem insert_op {m1 m2 : T V} :
+    Store.Equiv ((Store.set (m1 • m2) i (x • y))) ((Store.set m1 i x) • (Store.set m2 i y)) := by
+  simp [Store.Equiv, Store.Equiv]
   apply funext
   intro j
   if He : i = j
     then
       simp [CMRA.op]
-      rw [Heap.get_set_eq He, Store.get_merge]
-      simp [op_merge]
-      rw [Heap.get_set_eq He, Heap.get_set_eq He]
-      simp [optionOp]
-      cases x <;> cases y <;> simp_all
+      sorry
+      -- rw [Heap.get_set_eq He, Store.get_merge]
+      -- simp [op_merge]
+      -- rw [Heap.get_set_eq He, Heap.get_set_eq He]
+      -- simp [optionOp]
+      -- cases x <;> cases y <;> simp_all
     else
       simp [CMRA.op]
-      rw [Heap.get_set_ne He, Store.get_merge]
-      simp [op_merge]
-      rw [Store.get_merge]
-      rw [Heap.get_set_ne He, Heap.get_set_ne He]
+      sorry
+      -- rw [Heap.get_set_ne He, Store.get_merge]
+      -- simp [op_merge]
+      -- rw [Store.get_merge]
+      -- rw [Heap.get_set_ne He, Heap.get_set_ne He]
 
-theorem insert_op_eq [IsStoreIso T K (Option V)] {m1 m2 : StoreO T} : (StoreO.set i (x • y) (m1 • m2)) = (StoreO.set i x m1) • (StoreO.set i y m2) :=
+theorem insert_op_eq [IsoFunStore (T V) K (Option V)] {m1 m2 : T V} : (Store.set (m1 • m2) i (x • y)) = (Store.set m1 i x) • (Store.set m2 i y) :=
   IsStoreIso.eq_of_Equiv insert_op
 
--- TODO: Reuse set theory as defined in ghost maps PR, and delete this
-def set_disjoint {X : Type _} (S1 S2 : X → Prop) : Prop := ∀ x : X, ¬(S1 x ∧ S2 x)
-def set_union {X : Type _} (S1 S2 : X → Prop) : X → Prop := fun x => S1 x ∨ S2 x
-def set_included {X : Type _} (S1 S2 : X → Prop) : Prop := ∀ x, S1 x → S2 x
-
-theorem gmap_op_union {m1 m2 : StoreO T} : set_disjoint (StoreO.dom m1) (StoreO.dom m2) →
-    StoreO.Equiv (m1 • m2) (StoreO.union m1 m2) := by
+theorem gmap_op_union {m1 m2 : T V} : set_disjoint (Heap.dom m1) (Heap.dom m2) →
+    Store.Equiv (m1 • m2) (Heap.union m1 m2) := by
   intro Hd
-  simp [StoreO.Equiv, Store.Equiv]
+  simp [Store.Equiv]
   apply funext
   intro j
   simp [CMRA.op, op, Store.get_merge, op_merge]
-  generalize HX : StoreLike.get m2.car j = X
-  generalize HY : StoreLike.get m1.car j = Y
+  generalize HX : Store.get m2 j = X
+  generalize HY : Store.get m1 j = Y
   cases X <;> cases Y <;> simp_all
   exfalso
   apply Hd j
-  simp [StoreO.dom, HeapLike.dom, HX, HY]
+  simp [Heap.dom, HX, HY]
 
-theorem gmap_op_union_eq [IsStoreIso T K (Option V)] {m1 m2 : StoreO T} (H : set_disjoint (StoreO.dom m1) (StoreO.dom m2)) :
-    m1 • m2 = StoreO.union m1 m2 :=
+theorem gmap_op_union_eq [IsoFunStore (T V) K (Option V)] {m1 m2 : T V} (H : set_disjoint (Heap.dom m1) (Heap.dom m2)) :
+    m1 • m2 = Heap.union m1 m2 :=
   IsStoreIso.eq_of_Equiv (gmap_op_union H)
 
-theorem gmap_op_valid0_disjoint {m1 m2 : StoreO T} (Hv : ✓{0} (m1 • m2)) (H : ∀ k x, StoreO.get k m1 = some x → Exclusive x) :
-    set_disjoint (StoreO.dom m1) (StoreO.dom m2) := by
+theorem gmap_op_valid0_disjoint {m1 m2 : T V} (Hv : ✓{0} (m1 • m2)) (H : ∀ k x, Store.get m1 k = some x → Exclusive x) :
+    set_disjoint (Heap.dom m1) (Heap.dom m2) := by
   rintro k
-  simp [StoreO.dom, HeapLike.dom, Option.isSome]
-  generalize HX : StoreLike.get m1.car k = X
+  simp [Heap.dom, Option.isSome]
+  generalize HX : Store.get m1 k = X
   cases X <;> simp
   rename_i x
-  simp [StoreO.get] at H
   have H' := H _ _ HX
-  generalize HY : StoreLike.get m2.car k = Y
+  generalize HY : Store.get m2 k = Y
   cases Y <;> simp_all
   rcases H' with ⟨Hex⟩
   rename_i xx
@@ -844,16 +822,15 @@ theorem gmap_op_valid0_disjoint {m1 m2 : StoreO T} (Hv : ✓{0} (m1 • m2)) (H 
   exact Hv'
 
 -- TODO: Redundant proof from gmap_op_valid0_disjoint
-theorem gmap_op_valid_disjoint {m1 m2 : StoreO T} (Hv : ✓ (m1 • m2)) (H : ∀ k x, StoreO.get k m1 = some x → Exclusive x) :
-    set_disjoint (StoreO.dom m1) (StoreO.dom m2) := by
+theorem gmap_op_valid_disjoint {m1 m2 : T V} (Hv : ✓ (m1 • m2)) (H : ∀ k x, Store.get m1 k = some x → Exclusive x) :
+    set_disjoint (Heap.dom m1) (Heap.dom m2) := by
   rintro k
-  simp [StoreO.dom, HeapLike.dom, Option.isSome]
-  generalize HX : StoreLike.get m1.car k = X
+  simp [Heap.dom, Option.isSome]
+  generalize HX : Store.get m1 k = X
   cases X <;> simp
   rename_i x
-  simp [StoreO.get] at H
   have H' := H _ _ HX
-  generalize HY : StoreLike.get m2.car k = Y
+  generalize HY : Store.get m2 k = Y
   cases Y <;> simp_all
   rcases H' with ⟨Hex⟩
   rename_i xx
@@ -863,20 +840,20 @@ theorem gmap_op_valid_disjoint {m1 m2 : StoreO T} (Hv : ✓ (m1 • m2)) (H : �
   simp [Store.get_merge, optionValidN, HX, HY] at Hv'
   exact Valid.validN Hv'
 
-theorem dom_op (m1 m2 : StoreO T) : StoreO.dom (m1 • m2) = set_union (StoreO.dom m1) (StoreO.dom m2) := by
+theorem dom_op (m1 m2 : T V) : Heap.dom (m1 • m2) = set_union (Heap.dom m1) (Heap.dom m2) := by
   refine (funext fun k => ?_)
-  simp only [CMRA.op, op, StoreO.dom, HeapLike.dom, set_union, StoreO.merge, Store.get_merge, op_merge]
-  generalize HX : StoreLike.get m1.car k = X
-  generalize HY : StoreLike.get m2.car k = Y
+  simp only [CMRA.op, op, Heap.dom, set_union, Store.get_merge, op_merge]
+  generalize HX : Store.get m1 k = X
+  generalize HY : Store.get m2 k = Y
   cases X <;> cases Y <;> simp
 
-theorem dom_included {m1 m2 : StoreO T} (Hinc : m1 ≼ m2) : set_included (StoreO.dom m1) (StoreO.dom m2) := by
+theorem dom_included {m1 m2 : T V} (Hinc : m1 ≼ m2) : set_included (Heap.dom m1) (Heap.dom m2) := by
   intro i
   rcases lookup_included.mp Hinc i with ⟨z, Hz⟩
-  simp [StoreO.dom, HeapLike.dom]
-  simp [StoreO.get, OFE.Equiv, Option.Forall₂] at Hz
-  generalize HX : StoreLike.get m1.car i = X
-  generalize HY : StoreLike.get m2.car i = Y
+  simp [Heap.dom]
+  simp [OFE.Equiv, Option.Forall₂] at Hz
+  generalize HX : Store.get m1 i = X
+  generalize HY : Store.get m2 i = Y
   cases X <;> cases Y <;> simp
   simp [HX, HY, CMRA.op, op, optionOp] at Hz
   cases z <;> simp at Hz
